Weidenbach_Book/Bits_Natural.thy
@@ -1,0 +1,162 @@
+theory Bits_Natural
+imports IICF
+  "~~/src/HOL/Word/Bits_Bit"
+  "~~/src/HOL/Word/Bool_List_Representation"
+begin
+
+instantiation nat :: bits
+begin
+
+definition test_bit_nat :: \<open>nat \<Rightarrow> nat \<Rightarrow> bool\<close> where
+  "test_bit i j = test_bit (int i) j"
+
+definition lsb_nat :: \<open>nat \<Rightarrow> bool\<close> where
+  "lsb i = (int i :: int) !! 0"
+
+definition set_bit_nat :: "nat \<Rightarrow> nat \<Rightarrow> bool \<Rightarrow> nat" where
+  "set_bit i n b = nat (bin_sc n b (int i))"
+
+definition set_bits_nat :: "(nat \<Rightarrow> bool) \<Rightarrow> nat" where
+  "set_bits f =
+  (if \<exists>n. \<forall>n'\<ge>n. \<not> f n' then
+     let n = LEAST n. \<forall>n'\<ge>n. \<not> f n'
+     in nat (bl_to_bin (rev (map f [0..<n])))
+   else if \<exists>n. \<forall>n'\<ge>n. f n' then
+     let n = LEAST n. \<forall>n'\<ge>n. f n'
+     in nat (sbintrunc n (bl_to_bin (True # rev (map f [0..<n]))))
+   else 0 :: nat)"
+
+definition shiftl_nat where
+  "shiftl x n = nat ((int x) * 2 ^ n)"
+
+definition shiftr_nat where
+  "shiftr x n = nat (int x div 2 ^ n)"
+
+definition bitNOT_nat :: "nat \<Rightarrow> nat" where
+  "bitNOT i = nat (bitNOT (int i))"
+
+definition bitAND_nat :: "nat \<Rightarrow> nat \<Rightarrow> nat" where
+  "bitAND i j = nat (bitAND (int i) (int j))"
+
+definition bitOR_nat :: "nat \<Rightarrow> nat \<Rightarrow> nat" where
+  "bitOR i j = nat (bitOR (int i) (int j))"
+
+definition bitXOR_nat :: "nat \<Rightarrow> nat \<Rightarrow> nat" where
+  "bitXOR i j = nat (bitXOR (int i) (int j))"
+
+instance ..
+
+end
+
+
+lemma nat_shiftr[simp]:
+  "m >> 0 = m"
+  \<open>((0::nat) >> m) = 0\<close>
+  \<open>(m >> Suc n) = (m div 2 >> n)\<close> for m :: nat
+  by (auto simp: shiftr_nat_def zdiv_int zdiv_zmult2_eq[symmetric])
+
+lemma nat_shifl_div: \<open>m >> n = m div (2^n)\<close> for m :: nat
+  by (induction n arbitrary: m) (auto simp: div_mult2_eq)
+
+lemma nat_shiftl[simp]:
+  "m << 0 = m"
+  \<open>((0::nat) << m) = 0\<close>
+  \<open>(m << Suc n) = ((m * 2) << n)\<close> for m :: nat
+  by (auto simp: shiftl_nat_def zdiv_int zdiv_zmult2_eq[symmetric])
+
+lemma nat_shiftr_div2: \<open>m >> 1 = m div 2\<close> for m :: nat
+  by auto
+
+lemma nat_shiftr_div: \<open>m << n = m * (2^n)\<close> for m :: nat
+  by (induction n arbitrary: m) (auto simp: div_mult2_eq)
+
+export_code \<open>shiftl::nat \<Rightarrow> nat \<Rightarrow> nat\<close> checking SML
+value [nbe] \<open>shiftr (4::nat) 1\<close>
+
+definition shiftl1 :: \<open>nat \<Rightarrow> nat\<close> where
+  \<open>shiftl1 n = n << 1\<close>
+
+definition shiftr1 :: \<open>nat \<Rightarrow> nat\<close> where
+  \<open>shiftr1 n = n >> 1\<close>
+
+code_printing constant "shiftr1 :: nat \<Rightarrow> nat" \<rightharpoonup>
+  (SML) "(nat'_of'_integer(IntInf.~>>/ (integer'_of'_nat((_)),/ Word.fromInt 1)))" and
+  (SML_imp) "(nat'_of'_integer(IntInf.~>>/ (integer'_of'_nat((_)),/ Word.fromInt 1)))"
+
+code_printing constant "shiftl1 :: nat \<Rightarrow> nat" \<rightharpoonup>
+  (SML) "(nat'_of'_integer(IntInf.<</ (integer'_of'_nat((_)),/ Word.fromInt 1)))" and
+  (SML_imp) "(nat'_of'_integer(IntInf.<</ (integer'_of'_nat((_)),/ Word.fromInt 1)))"
+
+
+instantiation natural :: bits
+begin
+
+context includes natural.lifting begin
+
+lift_definition test_bit_natural :: \<open>natural \<Rightarrow> nat \<Rightarrow> bool\<close> is test_bit .
+
+lift_definition lsb_natural :: \<open>natural \<Rightarrow> bool\<close> is lsb .
+
+lift_definition set_bit_natural :: "natural \<Rightarrow> nat \<Rightarrow> bool \<Rightarrow> natural" is
+  set_bit .
+
+lift_definition set_bits_natural :: \<open>(nat \<Rightarrow> bool) \<Rightarrow> natural\<close>
+  is \<open>set_bits :: (nat \<Rightarrow> bool) \<Rightarrow> nat\<close> .
+
+lift_definition shiftl_natural :: \<open>natural \<Rightarrow> nat \<Rightarrow> natural\<close>
+  is \<open>shiftl :: nat \<Rightarrow> nat \<Rightarrow> nat\<close> .
+
+lift_definition shiftr_natural :: \<open>natural \<Rightarrow> nat \<Rightarrow> natural\<close>
+  is \<open>shiftr :: nat \<Rightarrow> nat \<Rightarrow> nat\<close> .
+
+lift_definition bitNOT_natural :: \<open>natural \<Rightarrow> natural\<close>
+  is \<open>bitNOT :: nat \<Rightarrow> nat\<close> .
+
+lift_definition bitAND_natural :: \<open>natural \<Rightarrow> natural \<Rightarrow> natural\<close>
+  is \<open>bitAND :: nat \<Rightarrow> nat \<Rightarrow> nat\<close> .
+
+lift_definition bitOR_natural :: \<open>natural \<Rightarrow> natural \<Rightarrow> natural\<close>
+  is \<open>bitOR :: nat \<Rightarrow> nat \<Rightarrow> nat\<close> .
+
+lift_definition bitXOR_natural :: \<open>natural \<Rightarrow> natural \<Rightarrow> natural\<close>
+  is \<open>bitXOR :: nat \<Rightarrow> nat \<Rightarrow> nat\<close> .
+
+end
+
+instance ..
+end
+
+context includes natural.lifting begin
+lemma [code]:
+  "integer_of_natural (m >> n) = (integer_of_natural m) >> n"
+  apply transfer
+  by (smt integer_of_natural.rep_eq msb_int_def msb_shiftr nat_eq_iff2 negative_zle
+      shiftr_int_code shiftr_int_def shiftr_nat_def shiftr_natural.rep_eq
+      type_definition.Rep_inject type_definition_integer)
+
+lemma [code]:
+  "integer_of_natural (m << n) = (integer_of_natural m) << n"
+  apply transfer
+  by (smt integer_of_natural.rep_eq msb_int_def msb_shiftl nat_eq_iff2 negative_zle
+      shiftl_int_code shiftl_int_def shiftl_nat_def shiftl_natural.rep_eq
+      type_definition.Rep_inject type_definition_integer)
+
+end
+
+
+lemma bitXOR_1_if_mod_2: \<open>bitXOR L 1 = (if L mod 2 = 0 then L + 1 else L - 1)\<close> for L :: nat
+  apply transfer
+  apply (subst int_int_eq[symmetric])
+  apply (rule bin_rl_eqI)
+   apply (auto simp: bitXOR_nat_def)
+  unfolding bin_rest_def bin_last_def bitXOR_nat_def
+       apply presburger+
+  done
+
+lemma bitAND_1_mod_2: \<open>bitAND L 1 = L mod 2\<close> for L :: nat
+  apply transfer
+  apply (subst int_int_eq[symmetric])
+  apply (subst bitAND_nat_def)
+   by (auto simp: zmod_int bin_rest_def bin_last_def bitval_bin_last[symmetric])
+
+end
